x_k = \frac{k}{n}



e_k =
\left\{
\begin{array}{ll}
    1 = ax_k + b\\
    0 = ax_{k-1} + b
\end{array}
\right.


y = \frac{x - x_{k-1}}{x_k - x_{k-1}}

y = nx - k + 1


e_k =
\left\{
\begin{array}{ll}
    1 = ax_k + b\\
    0 = ax_{k+1} + b
\end{array}
\right.


y=\frac{x - x_{k+1}}{x_k - x_{k+1}}

y = -nx + k + 1


y =
\left\{
\begin{array}{ll}
    1 + nx - k, \;\;\; x <    \frac{k}{n}\\[7pt]
    1 - nx + k, \;\;\; x \geq \frac{k}{n}
\end{array}
\right.

\;\;\Rightarrow\;\;

e_k = max(0,\;\; 1 - \left | nx - k \right |)



e'_k =
\left\{
\begin{array}{ll}
    0,\;\;\;\;\; e_k = 0\\[5pt]
    n,\;\;\;\;\; x < \frac{k}{n}\\[5pt]
    -n,\;\; x \geq \frac{k}{n}
\end{array}
\right.



\left\{
\begin{array}{ll}
    x \in [0, 1]\\[12pt]
    (a(x)u'(x))' + b(x)u'(x) + c(x)u(x) = f(x)\\[5pt]
    -a(0)u'(0) + \beta u(0) = \gamma\\[5pt]
    u(1) = u_1
\end{array}
\right.


B(u, v) = l(v)



{
B(u,v)=
- \beta v(0)u(0)\;
- \int_{0}^{1} a(x)v'(x)u'(x) \; dx \;
+ \int_{0}^{1} b(x)v(x)u'(x) \; dx \;
+ \int_{0}^{1} c(x)v(x)u(x) \; dx
}



{
l(v) = -\gamma v(0) + \int_{0}^{1} v(x) f(x) \; dx
}



a(x),\; b(x),\; c(x),\; f(x),\; \beta,\; \gamma,\; u_1